First hacked version of libm generator, lots of hardcoding and some cheats

tools/flover/semantics/expressionsLib.sml
@@ -1,0 +1,85 @@
+structure expressionsLib = struct
+
+  open HolKernel Abbrev ExpressionsTheory;
+  open RealArith realTheory realLib integerTheory intLib;
+
+  exception FloVerException of string;
+
+  val fvar_tm     = “Expressions$Var”
+  val fconst_tm   = “Expressions$Const”
+  val unop_tm     = “Expressions$Unop”
+  val bop_tm      = “Expressions$Binop”
+  val fma_tm      = “Expressions$Fma”
+  val downcast_tm = “Expressions$Downcast”
+
+  local fun err s = FloVerException ("Not a FloVer " ^ s) in
+  val dest_fvar     = HolKernel.dest_monop fvar_tm     $ err "var"
+  val dest_fconst   = HolKernel.dest_binop fconst_tm    $ err "const"
+  val dest_unop     = HolKernel.dest_binop unop_tm     $ err "unop"
+  val dest_bop      = HolKernel.dest_triop bop_tm      $ err "bop"
+  val dest_fma      = HolKernel.dest_triop fma_tm      $ err "fma"
+  val dest_downcast = HolKernel.dest_binop downcast_tm $ err "downcast"
+  end;
+
+  local fun getArgTy t = type_of t |> dest_type |> snd |> hd in
+  fun mk_fvar ty n = mk_comb (fvar_tm, n) |> inst [alpha |-> ty]
+  fun mk_fconst m c = list_mk_comb (inst [alpha |-> type_of c] fconst_tm, [m, c])
+  fun mk_unop u e =
+    list_mk_comb (inst [alpha |-> getArgTy e] unop_tm, [u, e])
+  fun mk_bop b e1 e2 =
+    list_mk_comb (inst [alpha |-> getArgTy e1] bop_tm, [b, e1, e2])
+  fun mk_fma e1 e2 e3 =
+    list_mk_comb (inst [alpha |-> getArgTy e1] fma_tm, [e1, e2, e3])
+  fun mk_downcast m e =
+    list_mk_comb (inst [alpha |-> getArgTy e] downcast_tm, [m, e])
+  end;
+
+  val is_fvar     = can dest_fvar
+  val is_fconst   = can dest_fconst
+  val is_unop     = can dest_unop
+  val is_bop      = can dest_bop
+  val is_fma      = can dest_fma
+  val is_downcast = can dest_downcast
+
+  fun realExp2ratExp (t:term) :term =
+    if type_of t = “:real expr” then
+      if is_fvar t then let
+        val var = dest_fvar t in
+        mk_fvar “:(int # int)” var end
+      else if is_fconst t then let
+        val (m,cst) = dest_fconst t
+        val (n,d) =
+          if realSyntax.is_div cst then
+            realSyntax.dest_div cst
+          else raise FloVerException ("Not a rational number" ^ (term_to_string cst))
+        val ni =
+          if realSyntax.is_real_literal n then
+            intSyntax.term_of_int $ realSyntax.int_of_term n
+          else raise FloVerException "Nominator not constant"
+        val di =
+          if realSyntax.is_real_literal d then
+            intSyntax.term_of_int $ realSyntax.int_of_term d
+          else raise FloVerException "Denominator not constant"
+        in
+          mk_fconst m (Parse.Term ‘(^ni, ^di)’) end
+      else if is_unop t then let
+        val (uop, e) = dest_unop t in
+        mk_unop uop (realExp2ratExp e) end
+      else if is_bop t then let
+        val (bop, e1, e2) = dest_bop t in
+        mk_bop bop (realExp2ratExp e1) (realExp2ratExp e2) end
+      else if is_fma t then let
+        val (e1, e2, e3) = dest_fma t in
+        mk_fma (realExp2ratExp e1) (realExp2ratExp e2) (realExp2ratExp e3) end
+      else if is_downcast t then let
+        val (m, e) = dest_downcast t in
+        mk_downcast m (realExp2ratExp e) end
+      else raise FloVerException ("Unsupported expression constructor in" ^ (term_to_string t))
+    else raise FloVerException "Not a real-valued expression";
+
+  fun realExp2ratExpConv t =
+    let val t_rat = realExp2ratExp t in
+      EVAL “^t = ratExp2realExp ^t_rat” |> REWRITE_RULE [EQ_CLAUSES]
+    end;
+
+end;
