libmGen/FloVerToCakeMLProofsScript.sml
@@ -1,0 +1,348 @@
+(*
+  Main connection theorem relating FloVer's roundoff error bound
+  to CakeML floating-point kernel executions
+*)
+(* HOL4 *)
+open machine_ieeeTheory realTheory realLib RealArith;
+(* CakeML *)
+open fpValTreeTheory fpSemTheory realOpsTheory semanticPrimitivesTheory
+     evaluateTheory ml_translatorTheory;
+(* Icing *)
+open floatToRealTheory FloVerToCakeMLTheory CakeMLtoFloVerProofsTheory;
+(* FloVer *)
+open ExpressionsTheory ExpressionSemanticsTheory CommandsTheory
+     EnvironmentsTheory IEEE_connectionTheory IEEE_reverseTheory
+     FloverMapTheory TypeValidatorTheory MachineTypeTheory;
+open preamble;
+
+val _ = new_theory "FloVerToCakeMLProofs";
+
+Definition usedVars_P_sound_def:
+  usedVars_P_sound e (env:(string,string,v) namespace) P =
+   ∀ x.
+     x IN domain (usedVars e) ⇒
+     ∃ fp.
+       nsLookup env (Short ("x" ++ (toString x))) = SOME (FP_WordTree fp) ∧
+       fp64_isFinite (compress_word fp) ∧
+       FST (P x) ≤ fp64_to_real (compress_word fp) ∧
+       fp64_to_real (compress_word fp) ≤ SND (P x)
+End
+
+Definition toFloVerEnv_def:
+  toFloVerEnv (env:(string,string,v) namespace) e =
+  λ (n:num).
+    case lookup n (usedVars e) of
+      NONE => NONE
+    | SOME () =>
+        case nsLookup env $ Short ("x" ++ (toString n)) of
+       | NONE => NONE
+       | SOME $ FP_WordTree fp => SOME $ compress_word fp
+       | SOME _ => NONE
+End
+
+Theorem approxEnv_toFloVerEnv:
+  ∀ (e:real expr) env P (Gamma:real expr -> mType option) (A:analysisResult).
+  usedVars_P_sound (e:real expr) env P ⇒
+  approxEnv (toREnv (toFloVerEnv env e)) Gamma A (usedVars e) LN (toREnv (toFloVerEnv env e))
+Proof
+  rpt strip_tac >> irule approxEnv_refl >> rw [toFloVerEnv_def, toREnv_def]
+  >- (
+    CASE_TAC >> gs[domain_lookup]
+    >- (CASE_TAC >> gs[])
+    >> Cases_on ‘lookup x (usedVars e)’ >> gs[])
+  >- (cheat) (* Needs validTypes assumption *)
+  >> gs[domain_lookup, usedVars_P_sound_def]
+  >> res_tac >> gs[]
+QED
+
+(*
+Theorem toFloVerEnv_rounded:
+  ∀ e flEnv P.
+    usedVars_P_sound e flEnv P ⇒
+    ∀ x v.
+      (toREnv (toFloVerEnv flEnv e)) x = SOME v ⇒
+      float_to_real ((real_to_float dmode v):(52,11) float) = v
+Proof
+  rw[toFloVerEnv_def, usedVars_P_sound_def]
+  >> gvs[CaseEqs ["option", "v", "lit"], domain_lookup,
+         fp64_to_real_def, real_to_fp64_def, fp64_to_float_float_to_fp64]
+  >> res_tac >> gvs[fp64_isFinite_def]
+  >> drule float_to_real_round_robin >> gs[]
+QED
+*)
+
+Theorem usedVars_P_sound_fVars_P_sound:
+  usedVars_P_sound e flEnv P ⇒
+  fVars_P_sound (usedVars e) (toREnv (toFloVerEnv flEnv e)) P
+Proof
+  rw[usedVars_P_sound_def, RealRangeArithTheory.fVars_P_sound_def,
+     toFloVerEnv_def, toREnv_def]
+  >> res_tac >> gs[domain_lookup, fp64_to_real_def]
+QED
+
+Definition real_env_rel_def:
+  real_env_rel (E:num -> word64 option) env vars =
+  ∀ x.
+    x IN vars ⇒
+    ∃ fp.
+      nsLookup env (Short $ STRCAT "x" (toString x)) = SOME (FP_WordTree fp) ∧
+      E x = SOME (compress_word fp)
+End
+
+Theorem FloVer_to_CML_real_sim:
+  ∀ e eReal prog st E env flEnv Gamma r fVars.
+    eReal = ratExp2realExp e ∧
+    SOME prog = toCmlRealExp e ∧
+    st.fp_state.real_sem ∧
+    real_env_rel E flEnv fVars ∧
+    domain $ usedVars e SUBSET fVars ∧
+    eval_expr (toREnv E) (toRTMap $ toRExpMap Gamma) (toREval eReal) r REAL ⇒
+    evaluate st (env with v := toRspace (nsAppend flEnv env.v)) [prog] =
+      (st, Rval [Real r])
+Proof
+  ho_match_mp_tac toCmlRealExp_ind >> rw[toCmlRealExp_def, ratExp2realExp_def]
+  >> gs[eval_expr_cases, toREval_def]
+  >> simp[Once evaluate_def]
+  >- (
+    gvs[real_env_rel_def, toREnv_def, CaseEqs["option", "v", "lit"]]
+    >> ‘i IN fVars’ by gs[Once usedVars_def, SUBSET_DEF]
+    >> res_tac
+    >> gvs[toRspace_def, namespacePropsTheory.nsLookup_nsMap,
+            namespacePropsTheory.nsLookup_nsAppend_some, fp64_to_real_def])
+  >- gvs[perturb_def, evaluate_def, do_app_def, state_component_equality]
+  >- (
+    gvs[CaseEq"option", evaluate_def]
+    >> rename1 ‘isCompat mR REAL’
+    >> Cases_on ‘mR’ >> gs[isCompat_def]
+    >> ‘domain (usedVars e) SUBSET fVars’ by (
+      qpat_x_assum ‘domain _ SUBSET _’ mp_tac
+      >> simp[Once usedVars_def])
+    >> last_x_assum $ drule_then drule
+    >> rpt $ disch_then drule
+    >> disch_then $ qspec_then ‘env’ assume_tac
+    >> gs[do_app_def, real_uop_def, getRealUop_def, evalUnop_def,
+          state_component_equality])
+  >- (
+    gvs[CaseEq"option", evaluate_def]
+    >> rename1 ‘isJoin mR1 mR2 REAL’
+    >> ‘mR1 = REAL ∧ mR2 = REAL’
+       by (
+         conj_tac >> irule eval_expr_real
+         >> once_rewrite_tac[CONJ_COMM] >> asm_exists_tac >> fs[]
+         >> rpt strip_tac
+         >> Cases_on ‘x’
+         >> fs[ExpressionAbbrevsTheory.toRTMap_def, option_case_eq])
+    >> rveq
+    >> rename1 ‘domain (usedVars (Binop bop e1 e2)) SUBSET fVars’
+    >> ‘domain (usedVars e1) SUBSET fVars ∧
+        domain (usedVars e2) SUBSET fVars’ by (
+      qpat_x_assum ‘domain _ SUBSET _’ mp_tac
+      >> simp[Once usedVars_def, domain_union])
+    >> rename1 ‘abs deltaOp ≤ mTypeToR REAL _’
+    >> ‘deltaOp = 0’ by gs[mTypeToR_def]
+    >> gvs[]
+    >> ntac 2 (
+      last_x_assum $ drule_then drule
+      >> rpt $ disch_then drule >> disch_then $ qspec_then ‘env’ assume_tac)
+    >> simp[Once evaluate_def, do_app_def, state_component_equality]
+    >> Cases_on ‘bop’
+    >> simp[real_bop_def, bopToRealBop_def, perturb_def, evalBinop_def])
+  >- (
+    gvs[CaseEq"option", evaluate_def]
+    >> rename1 ‘isJoin3 mR1 mR2 mR3 REAL’
+    >> ‘mR1 = REAL ∧ mR2 = REAL ∧ mR3 = REAL’
+       by (
+         rpt conj_tac >> irule eval_expr_real
+         >> once_rewrite_tac[CONJ_COMM] >> asm_exists_tac >> fs[]
+         >> rpt strip_tac
+         >> Cases_on ‘x’
+         >> fs[ExpressionAbbrevsTheory.toRTMap_def, option_case_eq])
+    >> rveq
+    >> rename1 ‘domain (usedVars (Fma e1 e2 e3)) SUBSET fVars’
+    >> ‘domain (usedVars e1) SUBSET fVars ∧ domain (usedVars e2) SUBSET fVars ∧
+        domain (usedVars e3) SUBSET fVars’ by (
+      qpat_x_assum ‘domain _ SUBSET _’ mp_tac
+      >> simp[Once usedVars_def, domain_union])
+    >> rename1 ‘abs deltaOp ≤ mTypeToR REAL _’
+    >> ‘deltaOp = 0’ by gs[mTypeToR_def]
+    >> gvs[]
+    >> ntac 3 (
+      last_x_assum $ drule_then drule
+      >> rpt $ disch_then drule >> disch_then $ qspec_then ‘env’ assume_tac)
+    >> simp[evaluate_def, do_app_def, state_component_equality, real_bop_def,
+            bopToRealBop_def, perturb_def, evalFma_def, evalBinop_def])
+QED
+
+Definition float_env_rel_def:
+  float_env_rel (E:num -> word64 option) env vars =
+  ∀ x v.
+    x IN vars ∧
+    E x = SOME v ⇒
+    ∃ fp.
+      nsLookup env (Short $ STRCAT "x" (toString x)) = SOME (FP_WordTree fp) ∧
+      v = compress_word fp
+End
+
+Theorem FloVer_to_CML_float_sim:
+  ∀ e prog st E env flEnv vF fVars.
+    SOME prog = toCmlFloatExp e ∧
+    st.fp_state.canOpt ≠ FPScope Opt ∧
+    domain $ usedVars e SUBSET fVars ∧
+    float_env_rel E flEnv fVars ∧
+    eval_expr_float (toFlExp e) E = SOME vF ⇒
+    ∃ fp.
+      evaluate st (env with v := nsAppend flEnv env.v) [prog] =
+      (st, Rval [FP_WordTree fp]) ∧
+      compress_word fp = vF
+Proof
+  ho_match_mp_tac toCmlFloatExp_ind >> rw[toCmlFloatExp_def]
+  >> gs[eval_expr_float_def, toFlExp_def]
+  >> simp[Once evaluate_def]
+  >- (
+    gvs[toFlEnv_def, float_env_rel_def, CaseEq"option"]
+    >> ‘i IN fVars’ by gs[Once usedVars_def, SUBSET_DEF]
+    >> res_tac
+    >> gvs[namespacePropsTheory.nsLookup_nsMap,
+            namespacePropsTheory.nsLookup_nsAppend_some])
+  >- gvs[perturb_def, evaluate_def, do_app_def, state_component_equality,
+         compress_word_def, real_to_fp64_def]
+  >- (
+    gvs[CaseEq"option", evaluate_def, astTheory.isFpBool_def]
+    >> ‘domain (usedVars e) SUBSET fVars’ by (
+      qpat_x_assum ‘domain _ SUBSET _’ mp_tac
+      >> simp[Once usedVars_def])
+    >> last_x_assum $ drule_then drule
+    >> rpt $ disch_then drule
+    >> disch_then $ qspec_then ‘env’ strip_assume_tac
+    >> gs[do_app_def, real_uop_def, getRealUop_def, evalUnop_def,
+          state_component_equality, semanticPrimitivesTheory.fp_translate_def,
+          compress_word_def, fp_uop_def, fp_uop_comp_def])
+  >- (
+    gvs[CaseEq"option", evaluate_def, astTheory.isFpBool_def]
+    >> rename1 ‘domain (usedVars (Binop bop e1 e2)) SUBSET fVars’
+    >> ‘domain (usedVars e1) SUBSET fVars ∧
+        domain (usedVars e2) SUBSET fVars’ by (
+      qpat_x_assum ‘domain _ SUBSET _’ mp_tac
+      >> simp[Once usedVars_def, domain_union])
+    >> ntac 2 (
+      last_x_assum $ drule_then drule
+      >> rpt $ disch_then drule >> disch_then $ qspec_then ‘env’ strip_assume_tac)
+    >> simp[do_app_def, state_component_equality, fp_translate_def]
+    >> Cases_on ‘bop’
+    >> gvs[fp_bop_def, fp_bop_comp_def, bopTofpBop_def, compress_word_def,
+           dmode_def])
+  >- (
+    gvs[CaseEq"option", evaluate_def, astTheory.isFpBool_def]
+    >> rename1 ‘domain (usedVars (Fma e1 e2 e3)) SUBSET fVars’
+    >> ‘domain (usedVars e1) SUBSET fVars ∧ domain (usedVars e2) SUBSET fVars ∧
+        domain (usedVars e3) SUBSET fVars’ by (
+      qpat_x_assum ‘domain _ SUBSET _’ mp_tac
+      >> simp[Once usedVars_def, domain_union])
+    >> ntac 3 (
+      last_x_assum $ drule_then drule
+      >> rpt $ disch_then drule >> disch_then $ qspec_then ‘env’ assume_tac)
+    >> gvs[evaluate_def, do_app_def, state_component_equality, fp_translate_def,
+           compress_word_def, fp_top_def, fp_top_comp_def, fpfma_def])
+QED
+
+Theorem FloVer_to_CML_float_sim_strong:
+  ∀ e prog st E env flEnv vF fVars.
+    SOME prog = toCmlFloatProg e ∧
+    domain $ usedVars e SUBSET fVars ∧
+    float_env_rel E flEnv fVars ∧
+    eval_expr_float (toFlExp e) E = SOME vF ⇒
+    ∃ fp.
+      evaluate st (env with v := nsAppend flEnv env.v) [prog] =
+      (st, Rval [FP_WordTree fp]) ∧
+      compress_word fp = vF
+Proof
+  rw[CaseEq"option", toCmlFloatProg_def]
+  >> simp[Once evaluate_def]
+  >> last_x_assum $ assume_tac o GSYM
+  >> drule FloVer_to_CML_float_sim
+  >> qmatch_goalsub_abbrev_tac ‘evaluate stN _ [p]’
+  >> ‘stN.fp_state.canOpt ≠ FPScope Opt’
+    by (unabbrev_all_tac >> COND_CASES_TAC >> gs[])
+  >> rpt $ disch_then $ drule
+  >> disch_then $ qspec_then ‘env’ strip_assume_tac >> gvs[]
+  >> unabbrev_all_tac >> gvs[state_component_equality, fpState_component_equality]
+  >> COND_CASES_TAC >> gvs[do_fpoptimise_def, compress_word_def]
+QED
+
+Theorem usedVars_ratExp2realExp:
+  ∀ e. usedVars e = usedVars $ ratExp2realExp e
+Proof
+  ho_match_mp_tac usedVars_ind >> rw[]
+  >> Cases_on ‘e’ >> gs[ratExp2realExp_def]
+  >- simp[usedVars_def]
+  >- (Cases_on ‘v’ >> simp[ratExp2realExp_def]
+      >> simp[usedVars_def])
+  >- (simp[Once usedVars_def] >> EVAL_TAC)
+  >- (simp[Once usedVars_def] >> EVAL_TAC)
+  >- (simp[Once usedVars_def] >> EVAL_TAC)
+  >- (simp[Once usedVars_def] >> EVAL_TAC)
+QED
+
+Theorem FloVer_CakeML_sound_error:
+  ∀ e eReal progReal progFloat flEnv A P defVars Gamma env E_real E_float
+      (st:'ffi semanticPrimitives$state).
+    eReal = ratExp2realExp e ∧
+    SOME progReal = toCmlRealExp e ∧
+    SOME progFloat = toCmlFloatProg eReal ∧
+    is64BitEval eReal ∧ noDowncast eReal ∧
+    is64BitEnv defVars ∧
+    CertificateChecker eReal A P defVars = SOME Gamma ∧
+    usedVars_P_sound eReal flEnv P ⇒
+  ∃ r fp err iv.
+    FloverMapTree_find eReal A = SOME (iv,err) ∧
+    (* the CakeML code returns a valid floating-point word *)
+    evaluate (empty_state with fp_state :=
+                empty_state.fp_state with
+                  <| real_sem := T; canOpt := FPScope NoOpt |>)
+             (env with v := toRspace (nsAppend flEnv env.v))
+             [progReal] =
+    (empty_state with fp_state :=
+       empty_state.fp_state with <| real_sem := T; canOpt := FPScope NoOpt |>,
+     Rval [Real r]) /\
+    evaluate st (env with v := (nsAppend flEnv env.v)) [progFloat] =
+      (st, Rval [FP_WordTree fp]) /\
+    (* the roundoff error is sound *)
+     real$abs (r - fp64_to_real (compress_word fp)) ≤ err
+Proof
+  rpt strip_tac
+  >> first_assum $ mp_then Any assume_tac usedVars_P_sound_fVars_P_sound
+  >> drule IEEE_reverseTheory.IEEE_connection_expr
+  >> rpt $ disch_then drule >> gs[SUBSET_REFL]
+  >> disch_then drule
+  >> disch_then $ qspec_then ‘toFloVerEnv flEnv eReal’ mp_tac
+  >> impl_tac
+  >- (drule approxEnv_toFloVerEnv >> gs[])
+  >> rpt strip_tac
+  >> first_x_assum $ irule_at Any
+  >> qmatch_goalsub_abbrev_tac ‘evaluate newSt (env with v := toRspace _) [_]’
+  >> ‘newSt.fp_state.real_sem’ by (unabbrev_all_tac >> gs[])
+  >> drule $ INST_TYPE [alpha |-> “:unit”] FloVer_to_CML_real_sim
+  >> rpt $ disch_then drule
+  >> disch_then $
+       qspecl_then [‘toFloVerEnv flEnv (ratExp2realExp e)’, ‘env’, ‘flEnv’,
+                    ‘Gamma’, ‘vR'’, ‘domain (usedVars e)’] mp_tac
+  >> impl_tac
+  >- (
+    rpt conj_tac >> gs[real_env_rel_def]
+    >> rpt strip_tac >> gs[usedVars_P_sound_def, usedVars_ratExp2realExp]
+    >> res_tac >> first_assum $ irule_at Any
+    >> gs[toFloVerEnv_def, domain_lookup])
+  >> disch_then $ irule_at Any
+  >> drule $ INST_TYPE [alpha|-> “:'ffi”] FloVer_to_CML_float_sim_strong
+  >> disch_then $ qspecl_then [‘st’,‘toFloVerEnv flEnv (ratExp2realExp e)’, ‘env’,
+                               ‘flEnv’, ‘vF’, ‘domain $ usedVars (ratExp2realExp e)’] mp_tac
+  >> impl_tac
+  >- (
+    unabbrev_all_tac
+    >> rw[float_env_rel_def, toFloVerEnv_def, CaseEqs["option", "v"]]
+    >> first_assum $ irule_at Any >> gs[])
+  >> strip_tac
+  >> gvs[]
+QED
+
+val _ = export_theory();
