libmGen/FloVerToCakeMLScript.sml
@@ -1,0 +1,118 @@
+(*
+  Translation from CakeML floating-point kernels to FloVer input
+*)
+
+(* HOL *)
+open binary_ieeeTheory machine_ieeeTheory lift_ieeeTheory;
+(* CakeML *)
+open astTheory;
+(* FloVer *)
+open ExpressionsTheory IEEE_connectionTheory;
+(* Dandelion *)
+open checkerDefsTheory;
+open preamble;
+
+val _ = new_theory "FloVerToCakeML";
+
+(** Translation from FloVer AST to CakeML AST **)
+Definition bopTofpBop_def:
+  bopTofpBop Expressions$Plus = FP_Add ∧
+  bopTofpBop Sub = FP_Sub ∧
+  bopTofpBop Mult = FP_Mul ∧
+  bopTofpBop Div = FP_Div
+End
+
+Definition toFloVerFloatExp_def:
+  toFloVerFloatExp (Expressions$Var i) = Expressions$Var i ∧
+  toFloVerFloatExp (Const m c) = Const M64 c ∧
+  toFloVerFloatExp (Unop Neg e) = Unop Neg (toFloVerFloatExp e) ∧
+  toFloVerFloatExp (Binop b e1 e2) =
+    Binop b (toFloVerFloatExp e1) (toFloVerFloatExp e2) ∧
+  toFloVerFloatExp (Fma e1 e2 e3) =
+    Fma (toFloVerFloatExp e1) (toFloVerFloatExp e2) (toFloVerFloatExp e3) ∧
+  toFloVerFloatExp (Downcast m e) =
+    Downcast M64 (toFloVerFloatExp e)
+End
+
+Definition toCmlFloatExp_def:
+  toCmlFloatExp (Expressions$Var i):ast$exp option =
+    SOME $ ast$Var (Short ("x" ++ (toString i))) ∧
+  toCmlFloatExp (Const M64 c) =
+    SOME $ App FpFromWord [Lit (Word64 (float_to_fp64 ((real_to_float dmode c):(52, 11) float)))] ∧
+  toCmlFloatExp (Unop Neg e) =
+    (case toCmlFloatExp e of
+    | NONE => NONE
+    | SOME e1 => SOME $ App (FP_uop FP_Neg) [e1]) ∧
+  toCmlFloatExp (Binop op e1 e2) =
+    (case toCmlFloatExp e1 of
+    | NONE => NONE
+    | SOME e1F =>
+      case toCmlFloatExp e2 of
+      | NONE => NONE
+      | SOME e2F =>
+        SOME $ App (FP_bop (bopTofpBop op)) [e1F; e2F]) ∧
+  toCmlFloatExp (Fma e1 e2 e3) =
+    (case toCmlFloatExp e1 of
+    | NONE => NONE
+    | SOME e1F =>
+      case toCmlFloatExp e2 of
+      | NONE => NONE
+      | SOME e2F =>
+        case toCmlFloatExp e3 of
+        | NONE => NONE
+        | SOME e3F =>
+          SOME $ App (FP_top FP_Fma) [e3F; e1F; e2F]) ∧
+  toCmlFloatExp _ = NONE
+End
+
+Definition toCmlFloatProg_def:
+  toCmlFloatProg e =
+  case toCmlFloatExp e of
+  | NONE => NONE
+  | SOME p => SOME $ FpOptimise NoOpt p
+End
+
+Definition bopToRealBop_def:
+  bopToRealBop Expressions$Plus = Real_Add ∧
+  bopToRealBop Sub = Real_Sub ∧
+  bopToRealBop Mult = Real_Mul ∧
+  bopToRealBop Div = Real_Div
+End
+
+Definition toCmlRealExp_def:
+  toCmlRealExp (Expressions$Var i):ast$exp option =
+    SOME $ ast$Var (Short ("x" ++ (toString i))) ∧
+  (** FIXME **)
+  toCmlRealExp (Const M64 (c,d)) =
+    SOME $ App (RealFromIntProd) [Lit (IntLit c); Lit (IntLit d)] ∧
+  toCmlRealExp (Unop Neg e) =
+    (case toCmlRealExp e of
+    | NONE => NONE
+    | SOME e1 => SOME $ App (Real_uop Real_Neg) [e1]) ∧
+  toCmlRealExp (Binop op e1 e2) =
+    (case toCmlRealExp e1 of
+    | NONE => NONE
+    | SOME e1R =>
+      case toCmlRealExp e2 of
+      | NONE => NONE
+      | SOME e2R =>
+        SOME $ App (Real_bop (bopToRealBop op)) [e1R; e2R]) ∧
+  toCmlRealExp (Fma e1 e2 e3) =
+    (case toCmlRealExp e1 of
+    | NONE => NONE
+    | SOME e1R =>
+      case toCmlRealExp e2 of
+      | NONE => NONE
+      | SOME e2R =>
+        case toCmlRealExp e3 of
+        | NONE => NONE
+        | SOME e3R =>
+          SOME $ App (Real_bop Real_Add) [App (Real_bop Real_Mul) [e1R; e2R]; e3R]) ∧
+  toCmlRealExp _ = NONE
+End
+
+Definition getPrecondFromCert_def:
+  getPrecondFromCert cert = λ (x:num). if x = 0 then SND (HD cert.iv) else (0,0:real)
+End
+
+val _ = export_theory ();
